ocaml/debruijn.ml
@@ -29,6 +29,10 @@ let rec convert (scope : scope) (e : named_expr) : expr =
     EReplace (make_ident id (lookup scope id), convert scope e1)
   | NAssign (id, e1) ->
     EAssign (make_ident id (lookup scope id), convert scope e1)
+  | NBorrow (rk, id) ->
+    EBorrow (rk, make_ident id (lookup scope id))
+  | NDeref e1 ->
+    EDeref (convert scope e1)
   | NCall (f, args) ->
     ECall (make_ident f 0, List.map (convert scope) args)
   | NLet (m, name, Some ty, e1, e2) ->
